Update toolchain, add and fix a test from Bhavik Mehta

MPL/PredTrans.lean
@@ -30,10 +30,14 @@ namespace MPL
 def PredTrans.Monotonic {ps : PostShape} {α : Type} (t : PostCond α ps → Assertion ps) : Prop :=
   ∀ Q₁ Q₂, (Q₁ ⊢ₚ Q₂) → (t Q₁) ⊢ₛ (t Q₂)
 
-/-- The of conjunction of a transformed precondition is the same as the transformed conjunction
-of preconditions. -/
+/-- Transforming a conjunction of postconditions is the same as the conjunction of transformed
+postconditions. -/
 def PredTrans.Conjunctive {ps : PostShape} {α : Type} (t : PostCond α ps → Assertion ps) : Prop :=
   ∀ Q₁ Q₂, t (Q₁ ∧ₚ Q₂) ⊣⊢ₛ t Q₁ ∧ t Q₂
+
+/-- Transforming the trivial postcondition yields the trivial precondition. -/
+def PredTrans.Conjunctive0 {ps : PostShape} {α : Type} (t : PostCond α ps → Assertion ps) : Prop :=
+  t (PostCond.partial (fun _ => ⌜True⌝)) ⊣⊢ₛ ⌜True⌝
 
 /-- Any predicate transformer that is conjunctive is also monotonic. -/
 def PredTrans.Conjunctive.mono {ps : PostShape} {α : Type}
@@ -54,12 +58,10 @@ def PredTrans.Conjunctive.mono {ps : PostShape} {α : Type}
 structure PredTrans (ps : PostShape) (α : Type) : Type where
   apply : PostCond α ps → Assertion ps
   conjunctive : PredTrans.Conjunctive apply
+  conjunctive0 : PredTrans.Conjunctive0 apply
 
 theorem PredTrans.mono {ps : PostShape} {α : Type} (t : PredTrans ps α) : PredTrans.Monotonic t.apply :=
   PredTrans.Conjunctive.mono t.apply t.conjunctive
-
-def PredTrans.const {ps : PostShape} {α : Type} (p : Assertion ps) : PredTrans ps α :=
-  ⟨fun _ => p, fun _ _ => SPred.and_self.symm⟩
 
 /--
   Given a fixed postcondition, the *stronger* predicate transformer will yield a
@@ -70,15 +72,19 @@ def PredTrans.le {ps : PostShape} {α : Type} (x y : PredTrans ps α) : Prop :=
 instance : LE (PredTrans ps α) := ⟨PredTrans.le⟩
 
 def PredTrans.pure {ps : PostShape} {α : Type} (a : α) : PredTrans ps α :=
-  { apply := fun Q => Q.1 a, conjunctive := by intro _ _; simp }
+  { apply := fun Q => Q.1 a, conjunctive := by intro _ _; simp, conjunctive0 := .rfl }
 
 def PredTrans.bind {ps : PostShape} {α β : Type} (x : PredTrans ps α) (f : α → PredTrans ps β) : PredTrans ps β :=
-  { apply := fun Q => x.apply (fun a => (f a).apply Q, Q.2), conjunctive := by
+  { apply := fun Q => x.apply (fun a => (f a).apply Q, Q.2),
+    conjunctive := by
       intro Q₁ Q₂
       apply SPred.bientails.of_eq
       dsimp
       conv => rhs; rw [← (x.conjunctive _ _).to_eq]
       conv in (f _).apply _ => rw [((f _).conjunctive _ _).to_eq]
+    conjunctive0 := by
+      apply SPred.bientails.of_eq
+      simp only [fun x => (f x).conjunctive0.to_eq, x.conjunctive0.to_eq]
   }
 
 instance : Monad (PredTrans ps) where
@@ -113,12 +119,18 @@ instance PredTrans.instLawfulMonad : LawfulMonad (PredTrans ps) :=
 -- The interpretation of `StateT σ (PredTrans ps) α` into `PredTrans (.arg σ ps) α`.
 -- Think: modifyGetM
 def PredTrans.pushArg {ps : PostShape} {σ : Type} {α : Type} (x : StateT σ (PredTrans ps) α) : PredTrans (.arg σ ps) α :=
-  { apply := fun Q s => (x s).apply (fun (a, s) => Q.1 a s, Q.2), conjunctive := by
+  { apply := fun Q s => (x s).apply (fun (a, s) => Q.1 a s, Q.2),
+    conjunctive := by
       intro Q₁ Q₂
       apply SPred.bientails.of_eq
       ext s
       dsimp
-      rw[← ((x s).conjunctive _ _).to_eq] }
+      rw [← ((x s).conjunctive _ _).to_eq],
+    conjunctive0 := by
+      apply SPred.bientails.of_eq
+      ext s
+      exact (x s).conjunctive0.to_eq
+  }
 
 def PredTrans.popArg {ps : PostShape} {α} (x : PredTrans (.arg σ ps) α) : StateT σ (PredTrans ps) α := fun s =>
   { apply Q := x.apply (fun r s' => Q.1 (r, s'), Q.2) s,
@@ -130,7 +142,13 @@ def PredTrans.popArg {ps : PostShape} {α} (x : PredTrans (.arg σ ps) α) : Sta
         rw[congrFun (x.conjunctive _ _).to_eq _]
       simp only [SPred.and] at this
       simp only [this]
-      rfl }
+      rfl
+    conjunctive0 := by
+      apply SPred.bientails.of_eq
+      simp only
+      conv in PredTrans.apply _ _ => apply x.conjunctive0.to_eq
+      rfl
+  }
 
 -- The interpretation of `ExceptT ε (PredTrans ps) α` into `PredTrans (.except ε ps) α`
 def PredTrans.pushExcept {ps : PostShape} {α ε} (x : ExceptT ε (PredTrans ps) α) : PredTrans (.except ε ps) α :=
@@ -142,7 +160,15 @@ def PredTrans.pushExcept {ps : PostShape} {α ε} (x : ExceptT ε (PredTrans ps)
       rw[← (x.conjunctive _ _).to_eq]
       congr
       ext x
-      cases x <;> simp }
+      cases x <;> simp
+    conjunctive0 := by
+      apply SPred.bientails.of_eq
+      conv => rhs; rw[← x.conjunctive0.to_eq]
+      dsimp
+      congr
+      ext x
+      cases x <;> simp
+  }
 
 def PredTrans.popExcept {ps : PostShape} {α} (x : PredTrans (.except ε ps) α) : ExceptT ε (PredTrans ps) α :=
   { apply Q := x.apply (fun a => Q.1 (.ok a), fun e => Q.1 (.error e), Q.2),
@@ -151,7 +177,13 @@ def PredTrans.popExcept {ps : PostShape} {α} (x : PredTrans (.except ε ps) α)
       apply SPred.bientails.of_eq
       dsimp
       rw[← (x.conjunctive _ _).to_eq]
-      rfl }
+      rfl
+    conjunctive0 := by
+      apply SPred.bientails.of_eq
+      conv => rhs; rw[← x.conjunctive0.to_eq]
+      dsimp
+      congr
+  }
 
 instance PredTrans.instMonadLiftArg : MonadLift (PredTrans m) (PredTrans (.arg σ m)) where
   monadLift x := PredTrans.pushArg (StateT.lift x)
